TA_More.thy
@@ -1,5 +1,5 @@
 theory TA_More
-  imports TA.Timed_Automata TA.DBM_Operations Refine_Imperative_HOL.IICF
+  imports TA.Timed_Automata TA.DBM_Operations Refine_Imperative_HOL.IICF "library/Graphs"
 begin
 
 chapter \<open>Mixed Additional Material on Timed Automata\<close>
@@ -49,14 +49,30 @@ lemma delay_V:
   "\<forall> c. (u \<oplus> d) c \<ge> 0" if "\<forall> c. u c \<ge> 0" "(d :: 't :: time) \<ge> 0"
   using that unfolding cval_add_def by auto
 
+context
+  notes [elim!]  = step.cases step'.cases step_t.cases step_z.cases
+begin
+
 lemma extend_ta_iff:
   "A \<turnstile> \<langle>l, u\<rangle> \<rightarrow> \<langle>l', u'\<rangle> \<longleftrightarrow> extend_ta A cs \<turnstile> \<langle>l, u\<rangle> \<rightarrow> \<langle>l', u'\<rangle>" if "\<forall> c. u c \<ge> 0"
   using that apply safe
      apply (force simp: extend_cc_iff reset_V intro: step_a.intros elim!: step_a.cases)
     apply (force simp add: extend_cc_iff delay_V)
-  apply (cases rule: step_a.cases, assumption)
+   apply (cases rule: step_a.cases, assumption)
+   apply (rule step.intros, rule step_a.intros)
+  unfolding extend_ta_def apply (force simp: trans_of_def)
+     apply assumption+
+  prefer 2
+  apply assumption
+  subgoal
+    by (metis extend_cc_iff inv_of_def prod.sel(2) reset_V)
+  subgoal
+    by (metis clock_val.intros delay_V extend_cc_iff inv_of_def prod.sel(2) step_t step_t.intros)
+  done
+    (*  apply simp
+apply (force simp add: extend_cc_iff)
    apply (auto simp add: reset_V extend_cc_iff intro: step_a.intros)
-  using extend_cc_iff delay_V by fast
+  using extend_cc_iff delay_V by fas *)
 
 lemma steps_iffI:
   "A \<turnstile> \<langle>l, u\<rangle> \<rightarrow>* \<langle>l', u'\<rangle> \<longleftrightarrow> A' \<turnstile> \<langle>l, u\<rangle> \<rightarrow>* \<langle>l', u'\<rangle>" if
@@ -64,19 +80,144 @@ lemma steps_iffI:
   "\<And> (A :: ('a, 'c, 't :: time, 's) ta) l u l' u'. A \<turnstile> \<langle>l, u\<rangle> \<rightarrow> \<langle>l', u'\<rangle> \<Longrightarrow> P u \<Longrightarrow> P u'" "P u" for
   A A' :: "('a, 'c, 't :: time, 's) ta"
   apply standard
-  apply (insert that(3))
+   apply (insert that(3))
   subgoal
     by (induction A\<equiv> A _ _ _ _ rule: steps.induct) (auto simp: that(1,2))
-   by (induction A\<equiv> A' _ _ _ _ rule: steps.induct) (auto simp: that(2) that(1)[symmetric])
+  by (induction A\<equiv> A' _ _ _ _ rule: steps.induct) (auto simp: that(2) that(1)[symmetric])
 
 lemma step_V:
   "\<forall> c. u' c \<ge> 0" if "A \<turnstile> \<langle>l, u\<rangle> \<rightarrow> \<langle>l', u'\<rangle>" "\<forall> c. u c \<ge> 0"
   using that by (auto simp: reset_V delay_V elim: step_a.cases)
 
+end (* End of context for aggressive elimination rules *)
+
 lemma extend_ta_iff_steps:
   "A \<turnstile> \<langle>l, u\<rangle> \<rightarrow>* \<langle>l', u'\<rangle> \<longleftrightarrow> extend_ta A cs \<turnstile> \<langle>l, u\<rangle> \<rightarrow>* \<langle>l', u'\<rangle>" if "\<forall> c. u c \<ge> 0"
   apply (intro steps_iffI extend_ta_iff)
     apply assumption
-   by (rule step_V, assumption+, rule that)
+  by (rule step_V, assumption+, rule that)
 
-end
+
+
+lemma collect_clkvt_alt_def:
+  "collect_clkvt T = \<Union>((set o fst \<circ> snd \<circ> snd \<circ> snd) ` T)"
+unfolding collect_clkvt_def by fastforce
+
+lemma ta_collect_clkt_alt_def:
+  "collect_clkt S = \<Union> (collect_clock_pairs ` (fst o snd) ` S)"
+unfolding Timed_Automata.collect_clkt_def by fastforce
+
+lemma ta_collect_clki_alt_def:
+  "collect_clki I = \<Union> (collect_clock_pairs ` I ` UNIV)"
+unfolding Timed_Automata.collect_clki_def by auto
+
+lemma constraint_clk_constraint_pair:
+  "constraint_clk ac = fst (constraint_pair ac)"
+by (cases ac) auto
+
+lemma collect_clks_inv_clk_set:
+  "collect_clks (inv_of A l) \<subseteq> clk_set A"
+  unfolding
+    clkp_set_def collect_clki_def collect_clks_def collect_clock_pairs_def
+  by (auto simp: constraint_clk_constraint_pair) blast
+
+lemma collect_clocks_clk_set:
+  assumes
+    "A \<turnstile> l \<longrightarrow>\<^bsup>g,a,r\<^esup> l'"
+  shows
+    "collect_clks g \<subseteq> clk_set A"
+  using assms unfolding clkp_set_def collect_clks_id collect_clkt_def by fastforce
+
+lemma reset_clk_set:
+  assumes
+    "A \<turnstile> l \<longrightarrow>\<^bsup>g,a,r\<^esup> l'"
+  shows
+    "set r \<subseteq> clk_set A"
+using assms by (fastforce simp: clkp_set_def collect_clkvt_def)
+
+lemma ac_iff:
+  "u1 \<turnstile>\<^sub>a ac \<longleftrightarrow> u2 \<turnstile>\<^sub>a ac" if
+  "u1 (fst (constraint_pair ac)) = u2 (fst (constraint_pair ac))"
+  using that by (cases ac) auto
+
+lemma ac_iff':
+  "u1 \<turnstile>\<^sub>a ac \<longleftrightarrow> u2 \<turnstile>\<^sub>a ac" if
+  "u1 (constraint_clk ac) = u2 (constraint_clk ac)"
+  using that by (cases ac) auto
+
+lemma cc_iff:
+  "u1 \<turnstile> cc \<longleftrightarrow> u2 \<turnstile> cc" if "\<forall> (c, d) \<in> collect_clock_pairs cc. u1 c = u2 c"
+  using that
+  by (auto 4 4
+      simp: ac_iff[of u1 _ u2] list_all_iff collect_clock_pairs_def
+      intro!: clock_val.intros
+      )
+
+lemma cc_iff':
+  "u1 \<turnstile> cc \<longleftrightarrow> u2 \<turnstile> cc" if "\<forall> c \<in> collect_clks cc. u1 c = u2 c"
+  using that
+  by (auto 4 4
+      simp: ac_iff'[of u1 _ u2] list_all_iff collect_clks_def
+      intro!: clock_val.intros
+      )
+
+lemma step_t_bisim:
+  "\<exists> u2'. A \<turnstile> \<langle>l, u2\<rangle> \<rightarrow>\<^bsup>d\<^esup> \<langle>l', u2'\<rangle> \<and> (\<forall> c. c \<in> clk_set A \<longrightarrow> u1' c = u2' c)"
+  if assms: "A \<turnstile> \<langle>l, u1\<rangle> \<rightarrow>\<^bsup>d\<^esup> \<langle>l', u1'\<rangle>" "\<forall> c. c \<in> clk_set A \<longrightarrow> u1 c = u2 c"
+  using that(1)
+  apply cases
+  apply (subst (asm) cc_iff'[of _ _ "u2 \<oplus> d"])
+  subgoal
+    using collect_clks_inv_clk_set[of A l] assms(2) by (auto simp: cval_add_def)
+  using assms(2) by (force simp: cval_add_def)
+
+lemma step_a_bisim:
+  "\<exists> u2'. A \<turnstile> \<langle>l, u2\<rangle> \<rightarrow>\<^bsub>a\<^esub> \<langle>l', u2'\<rangle> \<and> (\<forall> c. c \<in> clk_set A \<longrightarrow> u1' c = u2' c)"
+  if assms: "A \<turnstile> \<langle>l, u1\<rangle> \<rightarrow>\<^bsub>a\<^esub> \<langle>l', u1'\<rangle>" "\<forall> c. c \<in> clk_set A \<longrightarrow> u1 c = u2 c"
+  using that(1)
+  apply cases
+  subgoal for g r
+    apply (subst (asm) cc_iff'[of _ _ "u2"])
+    subgoal
+      using assms(2) by (force dest: collect_clocks_clk_set)
+    apply (subst (asm) (2) cc_iff'[of _ _ "[r\<rightarrow>0]u2"])
+    subgoal
+      apply rule
+      subgoal for c
+        using collect_clks_inv_clk_set[of A l'] assms(2) by (cases "c \<in> set r"; force)
+      done
+    apply (intro exI conjI)
+     apply (rule, assumption+)
+     apply (simp; fail)
+    apply rule
+    subgoal for c
+      using collect_clks_inv_clk_set[of A l'] assms(2) by (cases "c \<in> set r"; force)
+    done
+  done
+
+lemma step'_bisim:
+  "\<exists> u2'. A \<turnstile>' \<langle>l, u2\<rangle> \<rightarrow> \<langle>l', u2'\<rangle> \<and> (\<forall> c. c \<in> clk_set A \<longrightarrow> u1' c = u2' c)"
+  if assms: "A \<turnstile>' \<langle>l, u1\<rangle> \<rightarrow> \<langle>l', u1'\<rangle>" "\<forall> c. c \<in> clk_set A \<longrightarrow> u1 c = u2 c"
+  using that(1)
+  apply cases
+  apply (drule step_t_bisim[OF _ that(2)])
+  apply clarify
+  apply (drule step_a_bisim, assumption)
+  apply auto
+  done
+
+lemma ta_bisimulation:
+  "Bisimulation_Invariant
+  (\<lambda> (l, u) (l', u'). A \<turnstile>' \<langle>l, u\<rangle> \<rightarrow> \<langle>l', u'\<rangle>)
+  (\<lambda> (l, u) (l', u'). A \<turnstile>' \<langle>l, u\<rangle> \<rightarrow> \<langle>l', u'\<rangle>)
+  (\<lambda> (l, u) (l', u'). l' = l \<and> (\<forall> c. c \<in> clk_set A \<longrightarrow> u c = u' c))
+  (\<lambda> _. True) (\<lambda> _. True)
+  "
+  apply standard
+  subgoal for a b a'
+    by clarify (drule step'_bisim; auto)
+  subgoal for a b a'
+    by clarify (drule step'_bisim; auto)
+  ..
+
+end (* Theory *)
