library/Stream_More.thy
@@ -258,5 +258,46 @@ proof -
   then show ?thesis by blast
 qed
 
+lemma stream_all2_weaken:
+  "stream_all2 Q xs ys" if "stream_all2 P xs ys" "\<And> x y. P x y \<Longrightarrow> Q x y"
+  using that by (coinduction arbitrary: xs ys) auto
+
+lemma stream_all2_SCons1:
+  "stream_all2 P (x ## xs) ys = (\<exists>z zs. ys = z ## zs \<and> P x z \<and> stream_all2 P xs zs)"
+  by (subst (3) stream.collapse[symmetric], simp del: stream.collapse, force)
+
+lemma stream_all2_SCons2:
+  "stream_all2 P xs (y ## ys) = (\<exists>z zs. xs = z ## zs \<and> P z y \<and> stream_all2 P zs ys)"
+  by (subst stream.collapse[symmetric], simp del: stream.collapse, force)
+
+lemma stream_all2_shift1:
+  "stream_all2 P (xs1 @- xs2) ys =
+  (\<exists> ys1 ys2. ys = ys1 @- ys2 \<and> list_all2 P xs1 ys1 \<and> stream_all2 P xs2 ys2)"
+  apply (induction xs1 arbitrary: ys)
+   apply (simp; fail)
+  apply (simp add: stream_all2_SCons1 list_all2_Cons1)
+  apply safe
+  subgoal for a xs1 ys z zs ys1 ys2
+    by (inst_existentials "z # ys1" ys2; simp)
+  subgoal for a xs1 ys ys1 ys2 z zs
+    by (inst_existentials z "zs @- ys2" zs "ys2"; simp)
+  done
+
+lemma stream_all2_shift2:
+  "stream_all2 P ys (xs1 @- xs2) =
+  (\<exists> ys1 ys2. ys = ys1 @- ys2 \<and> list_all2 P ys1 xs1 \<and> stream_all2 P ys2 xs2)"
+  by (meson list.rel_flip stream.rel_flip stream_all2_shift1)
+
+lemma stream_all2_bisim:
+  assumes "stream_all2 op \<in> xs as" "stream_all2 op \<in> ys as" "sset as \<subseteq> S"
+  shows "stream_all2 (\<lambda> x y. \<exists> a. x \<in> a \<and> y \<in> a \<and> a \<in> S) xs ys"
+  using assms
+  apply (coinduction arbitrary: as xs ys)
+  subgoal for a u b v as xs ys
+    apply (rule conjI)
+     apply (inst_existentials "shd as", auto simp: stream_all2_SCons1; fail)
+    apply (inst_existentials "stl as", auto 4 3 simp: stream_all2_SCons1; fail)
+    done
+  done
 
 end
